theories/SLFWP.v
@@ -62,11 +62,19 @@ Lemma wp_weakest : forall t H Q,
   H ==> wp t Q.
 Proof using. introv M. rewrite <- wp_equiv. applys M. Qed.
 
-(** Note that the equivalence rule [wp_equiv] defines a unique
-    function [wp]: any two functions satisfying it are equal. *)
+(** As prove further in this chapter, it is possible to 
+    define a function [wp] satisfying [wp_equiv]. Formally: *)
 
 Definition wp_characterization (wp:trm->(val->hprop)->hprop) :=
   forall t H Q, (triple t H Q) <-> (H ==> wp t Q).
+
+Parameter wp_characterization_exists : exists wp0,
+  wp_characterization wp0.
+
+(** In fact, there are several ways in which [wp] can be defined.
+    It turns out that all possible definitions are equivalent.
+    In other words, [wp_equiv] defines a unique function.
+    We next formally justify this fact. *)
 
 Lemma wp_characterization_unique : forall wp1 wp2,
   wp_characterization wp1 ->
@@ -83,6 +91,296 @@ Proof using.
   applys himpl_antisym; applys L; auto.
 Qed.
 
+(** Thus, it really does not matter which definition of [wp] is
+    considered. Thereafter, we only exploit the characterization lemma
+    [wp_equiv], and never rely on the internal definition of [wp]. *)
+
+
+(* ******************************************************* *)
+(** ** Syntactic construction of a weakest precondition *)
+
+(** To carry out practical verification proofs, we introduce
+    a function [wpgen] that construct a weakest precondition
+    heap predicate expressed in terms of the Separation Logic
+    combinators, by induction on the structure of the program. *)
+
+Module WpgenAmbition.
+
+Parameter wpgen : trm -> (val->hprop) -> hprop.
+
+(** Intuitively, we'd like the "syntactic" function [wpgen]
+    to be provably equal to "semantic" function [wp].
+
+    In practice, to establish correctness of a program,
+    we only care for one direction of the implication: *)
+
+Parameter wpgen_sound : forall t Q,
+  wpgen t Q ==> wp t Q.
+
+(** If we manage to define such a function [wpgen], then we could
+    use [wpgen] to establish triples. *)
+
+Lemma triple_of_wpgen : forall H t Q,
+  H ==> wpgen t Q ->
+  triple t H Q.
+Proof using.
+  introv M. rewrite wp_equiv. hchange M. applys wpgen_sound.
+Qed.
+
+(** The reciprocal implication from [wp] to [wpgen] would be
+    interesting to have, as it would justify the completeness of [wpgen].
+    Completeness would show that any Separation Logic proof can be carried 
+    out using [wpgen]. Yet, it is not a priority to try to formalize this 
+    result in Coq for now. *)
+
+End WpgenAmbition.
+
+
+(* ******************************************************* *)
+(** ** Definition of formulae for terms *)
+
+(* ------------------------------------------------------- *)
+(** *** General structure *)
+
+(** [wpgen t] is defined by recursion on [t], as a function
+    that expects a postcondition [Q] and returns a [hprop].
+    We call "formula" the result type of [wgpen t]: *)
+
+Definition formula := (val->hprop) -> hprop.
+
+(** The general shape of the definition of [wpgen] is a
+    recursive function on [t], with recursive calls for
+    the subterms. The auxiliary functions named [wpgen_val],
+    [wpgen_if], etc... describe the body of [wpgen t] for
+    each term construct that [t] could be.
+
+[[
+  Fixpoint wpgen (t:trm) : formula :=
+    match t with
+    | trm_val v => wpgen_val v
+    | trm_seq t1 t2 => wpgen_seq (wpgen t1) (wpgen t2)
+    | trm_if t0 t1 t2 => wpgen_if (wpgen t0) (wpgen t1) (wpgen t2)
+    | ...
+    end.
+]]
+
+    In what follows, we present the definition of each of
+    these auxiliary functions.
+*)
+
+(* ------------------------------------------------------- *)
+(** *** Case of values *)
+
+(** First, consider a value [v]. The formula [wpgen (trm_val v)]
+    should be such that [H ==> wpgen (trm_val v) Q] entails
+    [triple (trm_val v) H Q]. Recall rule [triple_val]. *)
+
+Parameter triple_val : forall v H Q,
+  H ==> Q v ->
+  triple (trm_val v) H Q.
+
+(** [H ==> Q v] is a sufficient condition for [triple (trm_val v) H Q].
+    Thus, we wish [H ==> wpgen (trm_val v) Q] to imply [H ==> Q v],
+    for any [H]. To achieve this implication, it suffices to define
+    [wpgen (trm_val v) Q] as [Q v].
+
+    Recall that [wpgen_val v] describes the value of [wpgen (trm_val v)].
+    Thus, [wpgen_val v] is a function that takes [Q] as argument,
+    and returns the heap predicate [Q v]. *)
+
+Definition wpgen_val (v:val) : formula := fun Q =>
+  Q v.
+
+(** Just to be sure, let us check the desired property. *)
+
+Lemma triple_of_wpgen_val : forall v H Q,
+  H ==> wpgen_val v Q ->
+  triple (trm_val v) H Q.
+Proof using.
+  introv M. applys triple_val. unfolds wpgen_val. applys M.
+Qed.
+
+(** The pattern of the above lemma will be repeated for all terms.
+    To capture this pattern, let us say that a formula [F] is sound
+    for a term [t] iff [H ==> F Q] entails [triple t H Q]. *)
+
+Definition formula_sound_for (t:trm) (F:formula) : Prop :=
+  forall H Q, H ==> F Q -> triple t H Q.
+
+(** We can reformulate the lemma above as: *)
+
+Lemma wpgen_val_sound : forall v,
+  formula_sound_for (trm_val v) (wpgen_val v).
+Proof using. introv M. applys triple_of_wpgen_val M. Qed.
+
+
+(* ------------------------------------------------------- *)
+(** *** Case of sequences *)
+
+(** Second, consider a sequence [trm_seq t1 t2].
+    The formula [wpgen (trm_seq t1 t2)] should be such that
+    [H ==> [wpgen (trm_seq t1 t2)] Q] entails
+    [triple (trm_seq t1 t2) H Q].
+
+    Recall that [wpgen (trm_seq t1 t2)] evaluates to
+    [wpgen_seq (wpgen t1) (wpgen t2)]. The definition of
+    [wpgen_seq] can be derived from that of [triple_seq]. 
+    Recall that rule. *)
+
+Parameter triple_seq : forall t1 t2 H Q H1,
+  triple t1 H (fun r => H1) ->
+  triple t2 H1 Q ->
+  triple (trm_seq t1 t2) H Q.
+
+(** By induction hypothesis on the subterms, a [triple] for 
+    [t1] or [t2] is equivalent to a [wpgen] entailment. 
+    Replacing [triple t H Q] with [H ==> wp t Q] throughout
+    the rule [triple_seq] gives us: 
+
+[[
+    Parameter wgpen_seq1 : forall t1 t2 H Q H1,
+      H ==> wpgen t1 (fun r => H1) ->
+      H1 ==> wpgen t2 Q ->
+      H ==> wpgen_seq (wpgen t1) (wpgen t2) Q.
+]]
+
+    From there, let [F1] denote [wpgen t1] and [F2] denote [wpgen t2].
+    Moreover, let us substitute away [H1]. We obtain:
+
+[[
+  H => F1 (fun r => F2 Q) ->
+  wpgen_seq F1 F2
+]]
+
+    This leads us to the following definition of [wpgen_seq]. *)
+
+Definition wpgen_seq (F1 F2:formula) : formula := fun Q =>
+  F1 (fun X => F2 Q).
+
+(** Again, let us verify that we obtain the desired implication
+    for [trm_seq t1 t2], assuming that we have sound formulae
+    for the two subterms. *)
+
+Lemma wpgen_seq_sound : forall F1 F2 t1 t2,
+  formula_sound_for t1 F1 ->
+  formula_sound_for t2 F2 ->
+  formula_sound_for (trm_seq t1 t2) (wpgen_seq F1 F2).
+Proof using.
+  introv S1 S2 M. unfolds wpgen_seq. applys triple_seq.
+  { applys S1. applys M. }
+  { applys S2. applys himpl_refl. }
+Qed.
+
+
+(* ------------------------------------------------------- *)
+(** *** Case of let-bindings *)
+
+Fixpoint wpgen (t:trm) : formula :=
+  match t with
+  | trm_let x t1 t2 => wpgen_let (wpgen t1) (fun X => wpgen (subst x X t2))
+  end.
+
+
+Definition wpgen_let (F1:formula) (F2of:val->formula) : formula := fun Q =>
+  F1 (fun X => F2of X Q).
+
+
+(* ------------------------------------------------------- *)
+(** *** Case of variables *)
+
+Fixpoint wpgen (t:trm) : formula :=
+  match t with
+  | trm_var x => wpgen_fail
+  end.
+
+Definition wpgen_fail : formula := fun Q =>
+  \[False].
+
+Lemma wpgen_fail_sound : forall t,
+  formula_sound_for t wpgen_fail.
+
+
+(* ------------------------------------------------------- *)
+(** *** Case of applications *)
+
+Fixpoint wpgen (t:trm) : formula :=
+  match t with
+  | trm_app t1 t2 => wp t
+  ...
+  end.
+
+Lemma wp_sound : forall t,
+  formula_sound_for t (wp t).
+
+
+(* ------------------------------------------------------- *)
+(** *** Case of conditionals *)
+
+
+
+Definition wpgen_if_val (v:val) (F1 F2:formula) : formula := fun Q =>
+  \exists (b:bool), \[v = val_bool b] \* (if b then F1 Q else F2 Q).
+
+Definition wpgen_if (F0 F1 F2:formula) : formula :=
+  wpgen_let F0 (fun v => wpgen_if_val v F1 F2).
+
+
+(* ------------------------------------------------------- *)
+(** *** Taking the fixpoint *)
+
+Fixpoint wpgen (t:trm) : formula :=
+  match t with
+  | trm_val v => wpgen_val v
+  | trm_var x => wpgen_fail
+  | trm_fun x t1 => wpgen_val (val_fun x t1)
+  | trm_fix f x t1 => wpgen_val (val_fix f x t1)
+  | trm_if t0 t1 t2 => wpgen_if (wpgen t0) (wpgen t1) (wpgen t2)
+  | trm_let x t1 t2 => wpgen_let (wpgen t1) (fun X => wpgen (subst x X t2))
+  | trm_app t1 t2 => wgpen_app t1 t2
+  end.
+
+
+
+Fixpoint wpgen (E:ctx) (t:trm) : formula :=
+  let aux := wpgen E in
+  match t with
+  | trm_val v => wpgen_val v
+  | trm_var x => wpaux_var E x
+  | trm_fun x t1 => trm_fun (isubst (Ctx.rem x E) t1)
+  | trm_fix f x t1 => trm_fix (isubst (Ctx.rem x (Ctx.rem f E)) t1))
+  | trm_if t0 t1 t2 => wpgen_if (aux t0) (aux t1) (aux t2)
+  | trm_let x t1 t2 => wpgen_let (aux t1) (fun X => wpgen (Ctx.add x X E) t2)
+  | trm_app t1 t2 => wgpen_app (isubst E t1) (isubst E t2)
+  end.
+
+
+
+
+Lemma wpgen_himpl_wp : forall t Q,
+  H ==> wpgen t Q ->
+  triple t H Q.
+
+  H ==> wp t Q ->
+  triple t H Q.
+
+  H ==> wpgen t Q ->
+  H ==> wp t Q ->
+
+  wpgen t Q ==> wp t Q.
+
+(in details)
+
+then derive
+
+  Lemma triple_of_wpgen : forall t Q,
+    H ==> wpgen t Q ->
+    triple t H Q.
+
+
+
+
+(* ####################################################### *)
+(** * Additional contents *)
 
 (* ******************************************************* *)
 (** ** Semantic definition of weakest precondition *)
@@ -143,8 +441,6 @@ Proof using.
 (* /SOLUTION *)
 Qed.
 
-(** Thereafter, we will only exploit the characterization lemma
-    [wp_equiv], and never rely on the internal definition of [wp]. *)
 
 
 (* ******************************************************* *)
@@ -244,59 +540,6 @@ done.
 
 -------
 
-
-Definition wpgen_fail : formula := fun Q =>
-  \[False].
-
-Definition wpgen_val (v:val) : formula := fun Q =>
-  Q v.
-
-Definition wpgen_let (F1:formula) (F2of:val->formula) : formula := fun Q =>
-  F1 (fun X => F2of X Q).
-
-Definition wpgen_seq (F1 F2:formula) : formula := fun Q =>
-  F1 (fun X => F2 Q).
-
-Definition wpgen_app (t1:trm) (t2:trm) : formula := fun Q =>  
-  wp (trm_app t1 t2) Q.
-
-Definition wpgen_if_val (v:val) (F1 F2:formula) : formula := fun Q =>
-  \exists (b:bool), \[v = val_bool b] \* (if b then F1 Q else F2 Q).
-
-Definition wpgen_if (F0 F1 F2:formula) : formula :=
-  wpgen_let F0 (fun v => wpgen_if_val v F1 F2).
-
-Fixpoint wpgen (t:trm) : formula :=
-  match t with
-  | trm_val v => wpgen_val v
-  | trm_var x => wpgen_fail
-  | trm_fun x t1 => wpgen_val (val_fun x t1)
-  | trm_fix f x t1 => wpgen_val (val_fix f x t1)
-  | trm_if t0 t1 t2 => wpgen_if (wpgen t0) (wpgen t1) (wpgen t2)
-  | trm_let x t1 t2 => wpgen_let (wpgen t1) (fun X => wpgen (subst x X t2))
-  | trm_app t1 t2 => wgpen_app t1 t2
-  end.
-
-
-Lemma wpgen_himpl_wp : forall t Q,
-  H ==> wpgen t Q ->
-  triple t H Q.
-
-  H ==> wp t Q ->
-  triple t H Q.
-
-  H ==> wpgen t Q ->
-  H ==> wp t Q ->
-
-  wpgen t Q ==> wp t Q.
-
-(in details)
-
-then derive
-
-  Lemma triple_of_wpgen : forall t Q,
-    H ==> wpgen t Q ->
-    triple t H Q.
 
 
 
